\documentclass{ximera}

\input{../preamble.tex}

\author{Bart Snapp}

\title{Fields}

\begin{document}
\begin{abstract}
  We introduce fields.
\end{abstract}
\maketitle

\begin{definition}
  A \dfn{field} is a set $K$ with two operations that we will denote
  by $+$ and $\cdot$ such that the following properties hold:
  \begin{description}
  \item[Closure] If $a,b\in K$, then $a+b\in K$ and $a\cdot b\in K$.
  \item[Associativity] If $a,b,c\in K$, then
    \[
    a+(b+ c)  = (a+ b)+c\quad\text{and}\quad a\cdot(b\cdot c)  = (a\cdot b)\cdot c.
    \]
  \item[Commutativity] If $a,b\in K$, then
    \[
    a+b = b+a\quad\text{and}\quad a\cdot b = b\cdot a.
    \]
  \item[Identities] There exists $0,1\in K$ such that for all $a\in K$
    \[
    0+a = a + 0 = a \quad\text{and}\quad 1\cdot a = a\cdot 1 = a.
    \]
  \item[Inverses] For all $a\in K$, there exists $(-a)$, and if $a\ne
    0$, there exists $a^{-1}$ such that
    \[
    a+(-a) = (-a)+ a = 0\quad\text{and}\quad a\cdot a^{-1} = a^{-1}\cdot a  = 1.
    \]
  \item[Distributivity] If $a,b,c\in K$, then 
    \[
    a\cdot (b+c) = a\cdot b+ a\cdot c.
    \]
  \end{description}
\end{definition}


\begin{exercise}
  Let $K$ be a field. Prove that $(-1)\cdot a = (-a)$.
\end{exercise}



dfn, basic eg
\end{document}
